more switch examples

doc/tutorial/C/switch.c
@@ -2,10 +2,26 @@ int switch_test(int i) {
   
     switch(i) {
     case 0:
-       return 0 ;
+       return 0 ; break;
     case 1:
-      return 1 ;
+      return 1 ; break;
+    default : return 2;
     }
-    
-    return 2;
+}
+
+int twice (int n) {
+  switch (n) {
+  case 0: return 0;
+  case 1: n=2; return n;
+  case -1: n= -2; return n;
+  // case 3: n=n+0;
+  // default: n=n+n; break;
+  }
+  return n + n;
+}
+
+int f(unsigned int x) { switch (x) {
+   case 1: return 2; break;
+   case 2: case 3: case 0xffffffff: return 1; break;
+   default: return 1; }
 }
