doc/tutorial/vst_switch.v
@@ -4,7 +4,6 @@ Require Import VST.floyd.proofauto.
 Instance CompSpecs : compspecs. make_compspecs prog. Defined.
 Definition Vprog : varspecs. mk_varspecs prog. Defined.
 
-
 Open Scope program_scope.
 
 Definition switch_spec : ident * funspec :=
@@ -16,22 +15,84 @@ Definition switch_spec : ident * funspec :=
       SEP()
     POST [ tint ]
       PROP()
-      LOCAL(temp ret_temp (Vint (Int.repr (Int.signed i))))
-      SEP().
+      LOCAL(temp ret_temp (if Int.eq i Int.zero
+                           then Vint Int.zero
+                           else if Int.eq i Int.one
+                                then Vint Int.one
+                                else Vint (Int.repr 2)))
+                 SEP().
 
 Definition Gprog := ltac:(with_library prog [switch_spec]).
 
+     
 Lemma body_max: semax_body Vprog Gprog f_switch_test switch_spec.
 Proof.
   start_function.
-  forward_if True.
-  forward.
-  forward_if.
-  admit.
-  forward.
-  entailer!.
-  forward_if (i = 0 \/ i = 1 \/ (i <> 0 /\ i <> 1)).
-  forward.
-  forward_if.
-  
-  
+  forward_if ((@FF (environ->mpred) _));
+    forward; try entailer!.  
+  - replace (Int.eq i Int.zero) with true.
+    auto.
+    rewrite Int.signed_eq.
+    destruct zeq; intuition.
+  - repeat rewrite Int.signed_eq.
+    destruct zeq; intuition; simpl.
+    replace (Int.signed Int.zero) with 0 in * by auto with ints.
+    intuition.
+    destruct zeq; intuition.
+  - admit.
+Admitted.
+
+Require Import Clight.switch.
+
+Definition twice_spec :=
+  DECLARE _twice
+    WITH n : Z
+    PRE [ _n OF tint ]
+      PROP  (Int.min_signed <= n+n <= Int.max_signed)
+      LOCAL (temp _n (Vint (Int.repr n)))
+      SEP ()
+    POST [ tint ]
+      PROP ()
+      LOCAL (temp ret_temp (Vint (Int.repr (n+n))))
+      SEP ().
+
+
+Definition f_spec :=
+  DECLARE _f
+    WITH x : Z
+    PRE [ _x OF tuint ]
+      PROP  (0 <= x <= Int.max_unsigned)
+      LOCAL (temp _x (Vint (Int.repr x)))
+      SEP ()
+    POST [ tint ]
+      PROP ()
+      LOCAL (temp ret_temp (if (x =? 1) 
+                            then Vint (Int.repr 2) 
+                            else Vint (Int.repr 1)))
+      SEP ().
+
+
+Definition Gprog' : funspecs :=   ltac:(with_library prog [twice_spec]).
+
+Lemma body_twice: semax_body Vprog Gprog' f_twice twice_spec.
+Proof.
+start_function.
+forward_if (PROP() LOCAL(temp _n (Vint (Int.repr (n)))) SEP()).
+repeat forward; entailer!.
+repeat forward; entailer!.
+repeat forward; entailer!.
+repeat forward; entailer!.
+repeat forward; entailer!.
+repeat forward; entailer!.
+Qed.
+
+Lemma body_f: semax_body Vprog Gprog f_f f_spec.
+Proof.
+start_function.
+forward_if (@FF (environ->mpred) _).
+forward.
+forward.
+forward.
+forward.
+forward.
+Qed.
